split into modules (pt II, for real this time)

HOL_To_IMP_Minus/Refinements/HOL_To_IMP_Minus_Arithmetics.thy
@@ -30,448 +30,7 @@ declare mul_acc_nat.simps[simp del]
 case_of_simps mul_acc_nat_eq[simplified Nitpick.case_nat_unfold] : mul_acc_nat.simps
 compile_nat mul_acc_nat_eq basename mul_acc
 
-(* isolates the return value in its own subgoal *)
-lemma rewrite_terminates_with_res_IMP_Tailcall_value:
-  assumes "v = v'" and "terminates_with_res_IMP_Tailcall tc c s r v'"
-  shows "terminates_with_res_IMP_Tailcall tc c s r v"
-  using assms by blast
-
-(* isolates the function and its argument from a function application *)
-lemma rewrite_comb: assumes "f = g" "x = y" shows "f x = g y" using assms by blast
-
-ML\<open>
-
-structure GU = General_Util
-structure HTIB = HOL_To_IMP_Tactics_Base
-structure HTIU = HOL_To_IMP_Util
-structure HTIT = HOL_To_IMP_Tailcalls_Tactics
-structure TU = Tactic_Util
-structure SUT = State_Update_Tracking
-structure SUTIT = State_Update_Tracking_IMP_Tailcalls
-structure PU = Parse_Util
-
-structure Seq = HTIU.Seq
-
-infix 1 LET
-structure HTIU = struct
-open HTIU
-
-fun refl_tac ctxt = resolve_tac ctxt [@{thm refl}]
-
-fun uresolve_tac ctxt thms =
-  Standard_Unify_Resolve.unify_resolve_tac (Unify_Resolve_Args.PRM.r ()) thms [] ctxt
-
-
-(* evaluates the first element, offers it (or NONE) to f, then returns a new sequence where the
-    evaluation of the first element has been memoized *)
-fun seq_peek1 f s =
-  case Seq.pull s of
-    SOME (x, xs) => (f (SOME x); Seq.cons x xs)
-  | NONE => (f NONE; Seq.empty)
-
-fun seq_peek_empty f = seq_peek1 (fn NONE => f () | SOME _ => ())
-
-structure Let = struct
-  fun x LET f = f x
-end
-
-end
-
-structure HTIB = struct
-
-(* find theorems of the form "f x = ...", given f possibly applied to some arguments *)
-type HOL_eqs_retrieval = Proof.context -> term -> thm list option
-(* FIXME: create a more robust filter *)
-fun get_HOL_eqs ctxt t =
-  let val thms = Find_Theorems.find_theorems ctxt NONE NONE true [
-      (* search for the head constant *)
-      (true, Find_Theorems.Pattern (head_of t)),
-      (* ignore conditional rules *)
-      (false, Find_Theorems.Pattern @{term "(\<Longrightarrow>)"})
-    ] |> snd |> map snd
-  in if null thms then NONE else SOME thms end
-
-(* SIMPS_TO helper tactics *)
-(* TODO: move into Util ? *)
-
-fun SIMPS_TO_tac simps ctxt =
-  TU.TRY' (simp_tac (ctxt addsimps simps))
-  THEN' resolve_tac ctxt [@{thm SIMPS_TOI}]
-
-fun SIMPS_TO_UNIF_tac simps ctxt =
-  resolve_tac ctxt [@{thm SIMPS_TO_UNIFI}]
-  THEN' TU.TRY' (SIMPS_TO_tac simps ctxt)
-  THEN' resolve_tac ctxt [@{thm reflexive}]
-
-(* helpers for updating and retrieving protected STATEs *)
-
-val STATE_interp_state_State_thms = @{thms STATE_eq interp_state_State_eq}
-
-fun SIMPS_TO_UNIF_STATE_interp_state_State_tac ctxt =
-  SIMPS_TO_UNIF_tac STATE_interp_state_State_thms ctxt
-
-fun STATE_interp_update_eq_STATE_interp_fun_upd ctxt =
-  resolve_tac ctxt [@{thm STATE_interp_update_eq_STATE_interp_fun_updI}]
-  THEN' SIMPS_TO_UNIF_STATE_interp_state_State_tac ctxt
-
-fun STATE_interp_retrieve_key_eq_tac finish_eq_tac ctxt = (* TODO: kind of ugly *)
-  resolve_tac ctxt [@{thm STATE_interp_retrieve_key_eqI}]
-  THEN' SIMPS_TO_UNIF_STATE_interp_state_State_tac (ctxt addsimps STATE_interp_state_State_thms)
-  THEN' finish_eq_tac
-
-(* tactics for assign, seq, and if that run one step of the program, given the appropriate theorems *)
-
-(* applies a theorem of the form, solving the first premise:
-   assumes "s' = s(k := ?val aexp s)"
-   and "s' r = val"
-   shows "?P (?assign k aexp) s r val" *)
-fun assign_tac thms ctxt =
-  resolve_tac ctxt thms
-  THEN' STATE_interp_update_eq_STATE_interp_fun_upd ctxt
-
-(* applies a theorem of the form:
-   assumes "?P1 c1" and "?P2 c2" shows "?P (?seq c1 c2)" *)
-fun seq_tac thms ctxt = resolve_tac ctxt thms
-
-fun if_tac thms ctxt =
-  resolve_tac ctxt thms
-  THEN' STATE_interp_retrieve_key_eq_tac (simp_tac ctxt) ctxt
-  THEN' SIMPS_TO_UNIF_STATE_interp_state_State_tac ctxt
-  THEN' SIMPS_TO_UNIF_STATE_interp_state_State_tac ctxt
-
-fun call_tac thms ctxt correctness =
-  resolve_tac ctxt thms
-  (* solve correctness assumption *)
-  THEN' resolve_tac ctxt correctness
-  (* solve state update assumption: s' = s(r := val) *)
-  THEN' STATE_interp_update_eq_STATE_interp_fun_upd ctxt
-
-(* run one (seq assign ...), (seq call ...), or if step of a program *)
-fun run_step_tac seq_tac assign_tac call_tac if_tac =
-  (seq_tac THEN' (assign_tac ORELSE' call_tac))
-  ORELSE' if_tac
-
-val run_tac = REPEAT_ALL_NEW oooo run_step_tac
-
-end
-
-structure HTIT = struct
-
-val logger = Logger.setup_new_logger HOL_to_IMP_base_logger "HOL_To_IMP_Tailcall_Tactics"
-
-
-(* destructors for IMP-Tailcalls *)
-
-type terminates_with_res_IMP_Tailcall_args = {tc: term, c: term, s: term, r: term, v: term}
-type terminates_with_IMP_Tailcall_args = {tc: term, c: term, s: term, s': term}
-
-val dest_terminates_with_res_IMP_Tailcall =
-  \<^Const_fn>\<open>terminates_with_res_IMP_Tailcall for tc c s r v => \<open>{tc = tc, c = c, s = s, r = r, v = v}\<close>\<close>
-val dest_terminates_with_res_IMP_Tailcall_prop =
-  HTIU.dest_Trueprop #> dest_terminates_with_res_IMP_Tailcall
-
-val dest_terminates_with_IMP_Tailcall =
-  \<^Const_fn>\<open>terminates_with_IMP_Tailcall for tc c s s' => \<open>{tc = tc, c = c, s = s, s' = s'}\<close>\<close>
-val dest_terminates_with_IMP_Tailcall_prop =
-  HTIU.dest_Trueprop #> dest_terminates_with_IMP_Tailcall
-
-fun with_dest_tac msg dest tac =
-  let fun wrap_tac concl =
-    case try dest concl of
-      NONE => (writeln msg; K no_tac)
-    | SOME x => tac x
-  in TU.SUBGOAL_STRIPPED (snd o snd) wrap_tac end
-
-val with_dest_terminates_with_res_IMP_Tailcall_prop =
-  with_dest_tac "couldn't find dest_terminates_with_res_IMP_Tailcall in conclusion"
-    dest_terminates_with_res_IMP_Tailcall_prop
-
-val with_dest_terminates_with_IMP_Tailcall_prop =
-  with_dest_tac "couldn't find dest_terminates_with_IMP_Tailcall in conclusion"
-    dest_terminates_with_IMP_Tailcall_prop
-
-
-(* destructors for IMP-Minus *)
-
-val dest_terminates_with_res_IMP_Minus =
-  \<^Const_fn>\<open>terminates_with_res_IMP_Minus for c s r v => \<open>(c, s, r, v)\<close>\<close>
-
-val dest_tailcall_to_IMP_Minus =
-  \<^Const_fn>\<open>tailcall_to_IMP_Minus for c => c\<close>
-
-val dest_terminates_with_res_IMP_Minus_tailcall_to_IMP_Minus =
-  dest_terminates_with_res_IMP_Minus #> (fn (c, _, _, _) => c) #> dest_tailcall_to_IMP_Minus
-
-val dest_terminates_with_res_IMP_Minus_tailcall_to_IMP_Minus_prop =
-  HTIU.dest_Trueprop #> dest_terminates_with_res_IMP_Minus_tailcall_to_IMP_Minus
-
-
-(* starting tactics *)
-
-fun preprocess_tac get_IMP_def =
-  let fun tac ctxt conclusion =
-    case try dest_terminates_with_res_IMP_Minus_tailcall_to_IMP_Minus_prop conclusion of
-      NONE =>
-        (@{log Logger.WARN} ctxt (fn _ => Pretty.block [
-          Pretty.str "Could not find ",
-          Syntax.pretty_term ctxt @{term tailcall_to_IMP_Minus},
-          Pretty.str " big step in conclusion ",
-          Syntax.pretty_term ctxt conclusion
-        ] |> Pretty.string_of);
-        K no_tac)
-      | SOME c =>
-        let val solve_simple_goal_tac =
-          (EqSubst.eqsubst_tac ctxt [0] (get_IMP_def ctxt c |> the_list)
-          THEN' Simplifier.simp_tac ctxt)
-          |> SOLVED'
-        in
-          resolve_tac ctxt [@{thm terminates_with_res_IMP_Minus_if_terminates_with_res_IMP_TailcallI}]
-          (* solve the invariant: invar f_IMP_tailcall *)
-          THEN' solve_simple_goal_tac
-          (* solve the assumption: ''f.ret'' in vars f_IMP_tailcall *)
-          THEN' solve_simple_goal_tac
-        end
-  in TU.SUBGOAL_STRIPPED (snd o snd) o tac end
-
-fun flip_eq_thm ctxt thm = Thm.proof_attributes [Calculation.symmetric] thm ctxt |> fst
-
-val rewrite_eq_state_retrieval_sym_tac =
-  let
-    fun rewrite_focused_tac {prems, context = ctxt, ...} =
-      let val prems_flipped = map (flip_eq_thm ctxt) prems
-      in
-        REPEAT_ALL_NEW (HTIU.subst_first_tac ctxt prems_flipped)
-        THEN' TU.insert_tac prems_flipped ctxt
-      end
-    fun rewrite_tac ctxt prems {s, ...}  =
-      let
-        val is_eq_state_retrieval_prem =
-          GU.try_bool
-            (HTIU.dest_Trueprop #>
-            \<^Const_fn>\<open>HOL.eq _ for _ s_app => \<open>SUT.is_state_state_retrieval s s_app\<close>\<close>)
-        val eq_state_retrieval_prems = GU.find_indices is_eq_state_retrieval_prem prems
-      in
-        TU.focus_delete_prems_tac (HTIU.successors eq_state_retrieval_prems)
-          rewrite_focused_tac ctxt
-      end
-  in
-    TU.FOCUS_PARAMS_CTXT' (
-      TU.SUBGOAL_STRIPPED (fst o snd) o (
-        with_dest_terminates_with_res_IMP_Tailcall_prop oo rewrite_tac))
-  end
-
-fun setup_induction_tac get_inducts =
-  let fun focused_tac ctxt {s, v, ...} =
-    let
-      (* v is of the form f (s ''...'') (s ''...'') ..., where f is the HOL function we are after *)
-      val head = head_of v
-      val instantiations =
-        head |> dest_Const |> fst
-        |> Compile_Nat.get_compiled_const (Context.Proof ctxt) |> #arg_regs
-        |> map (HOL_To_IMP_Util.mk_state_register_retrieval s)
-        |> map (fn t => SOME (NONE, (t, false)))
-      val arbitrary = [dest_Free s]
-      val inducts = get_inducts ctxt head
-    in
-      Induction.induction_tac ctxt true [instantiations] [arbitrary] [] inducts []
-      (* needed for inductions of functions defined on pattern matching; they create equalities of the
-         form "t = s ''<register>''", which have to be rewritten in the goal's conclusion" *)
-      THEN_ALL_NEW (TU.TRY' (rewrite_eq_state_retrieval_sym_tac ctxt))
-    end
-  in TU.FOCUS_PARAMS_CTXT' (with_dest_terminates_with_res_IMP_Tailcall_prop o focused_tac) end
-
-fun start_case_tac get_IMP_def =
-  let fun focused_tac ctxt {c, ...} =
-    EqSubst.eqsubst_tac ctxt [2] (get_IMP_def ctxt c |> the_list)
-    THEN' resolve_tac ctxt [@{thm terminates_with_res_IMP_Tailcall_start}]
-  in TU.FOCUS_PARAMS_CTXT' (with_dest_terminates_with_res_IMP_Tailcall_prop o focused_tac) end
-
-
-(* tactics for tAssign, tSeq, and tIf that run one step of the tailcall program *)
-
-val terminates_with_res_tAssign_tac = HTIB.assign_tac [@{thm terminates_with_res_tAssignI}]
-val terminates_with_res_tSeq_tac = HTIB.seq_tac [@{thm terminates_with_res_tSeqI}]
-val terminates_with_res_tIf_tac = HTIB.if_tac [@{thm terminates_with_res_tIf_processedI}]
-
-
-(* tactics for tAssign and tCall that handle terminates_with (instead of terminates_with_res) *)
-
-val terminates_with_tAssign_tac = HTIB.assign_tac [@{thm terminates_with_tAssignI}]
-
-fun terminates_with_tCall_tac get_func_corrects =
-  let fun tac ctxt {c, ...} =
-    case c of
-      Const (@{const_name tCall}, _) $ com $ _ =>
-        (case get_func_corrects ctxt com of
-            NONE => (writeln "no correctness found"; K no_tac (* TODO: error message *))
-          | SOME cs => HTIB.call_tac [@{thm terminates_with_tCallI}] ctxt cs)
-    | _ => K no_tac
-  in with_dest_terminates_with_IMP_Tailcall_prop o tac end
-
-(* given a constant term like eq_IMP, returns a list of potentially suitable IMP- correctness theorems *)
-fun get_func_corrects ctxt t =
-  let
-    open Find_Theorems
-    val thms = find_theorems ctxt NONE NONE true [
-      (* search for the equality theorem *)
-      (true, Pattern (@{term terminates_with_res_IMP_Minus} $ t (* TODO: wildcard for remaining args? *))),
-      (* ignore conditional rules *)
-      (false, Pattern @{term "(\<Longrightarrow>)"})
-    ] |> snd |> map snd
-  in if null thms then NONE else SOME thms end
-
-(* run a tailcall program to completion,
-   ends with terminates_with_res _ c _ _ _, where c is either an assignment, or tTAIL *)
-fun run_tac get_func_corrects ctxt =
-  HTIB.run_tac
-    (terminates_with_res_tSeq_tac ctxt)
-    (terminates_with_tAssign_tac ctxt)
-    (terminates_with_tCall_tac get_func_corrects ctxt)
-    (terminates_with_res_tIf_tac ctxt)
-
-
-(* finishing tactics *)
-
-val finish_tail_tac =
-  let
-    open Seq.M
-    open HTIU.Let
-
-    (* get a list of theorems of the form t_i = s ''reg_i'',
-       one for each argument in the function application term v *)
-    fun get_reg_eq_thms ctxt arg_reg_eq_tac s v =
-      (* v is of the form f t1 t2 ..., where f is the relevant HOL function;
-         extract the head f, and the terms t1, t2, ... *)
-      Term.strip_comb v
-      LET (fn (head, arg_terms) =>
-        (* fetch the compiled constant *)
-        Basics.try (dest_Const #> fst #> Compile_Nat.get_compiled_const (Context.Proof ctxt)) head
-        |> HTIU.seq_of_opt (fn () => writeln "could not load compiled constant" (* todo msg *))
-      BIND (fn {arg_regs, ...} =>
-        (* construct equalities of the form t_i = s ''reg_i'' *)
-        map2
-          (fn t => fn reg =>
-            HTIU.mk_eq (t, HTIU.mk_state_register_retrieval s reg)
-            |> HTIU.mk_Trueprop |> Thm.cterm_of ctxt)
-          arg_terms arg_regs
-      LET (fn arg_reg_eqs =>
-        (* prove the equalities *)
-        arg_reg_eqs |> List.map (TU.HEADGOAL (TU.apply_tac arg_reg_eq_tac)) |> Seq.A.sequence
-        (* this might not be an actual warning: if we simplify the HOL call incorrectly, a backtrack would be ok *)
-        |> HTIU.seq_peek_empty (fn () => writeln "could not prove one or more register equalities")
-      )))
-
-    (* tactic for proving the equalities: add existing premises, then simp *)
-    fun arg_reg_eq_tac ctxt prems =
-      Tactic.cut_facts_tac prems
-      THEN'
-      (* TODO: narrow down the simpset here... or come up with a better tactic *)
-      Simplifier.asm_simp_tac (
-        Simplifier.clear_simpset ctxt
-        addsimps @{thms STATE_eq interp_update_state_eq interp_state_State_eq})
-      THEN' Simplifier.asm_simp_tac ctxt
-
-    (* rewrite each argument t_i to s ''reg_i'' *)
-    fun rewrite_conclusion_arguments_tac ctxt arg_reg_eq_thms =
-      let
-        (* each argument is first drawn out into a separate subgoal t_i = ?v s
-           to prevent substitution from occurring inside s *)
-        fun rewrite_args_tac [] = HTIU.refl_tac ctxt
-          | rewrite_args_tac (thm :: thms) =
-              HTIU.uresolve_tac ctxt [@{thm rewrite_comb}]
-              THEN' rewrite_args_tac thms
-              THEN' HTIU.subst_first_tac ctxt [thm] THEN' HTIU.refl_tac ctxt
-      in
-        resolve_tac ctxt [@{thm rewrite_terminates_with_res_IMP_Tailcall_value}]
-        THEN' rewrite_args_tac (rev arg_reg_eq_thms)
-      end
-
-    fun solve_with_ih_tac ctxt prems s arg_reg_eq_thms =
-      let
-        val is_ih = Thm.concl_of #> can dest_terminates_with_res_IMP_Tailcall_prop
-
-        val instantiate_apply_ih_tac =
-          filter is_ih prems
-          |> map_filter (try (Drule.infer_instantiate' ctxt [SOME (Thm.cterm_of ctxt s)]))
-          |> resolve_tac ctxt
-
-        val solve_ih_prem_tac =
-          Tactic.cut_facts_tac prems
-          THEN' TU.TRY' (HTIU.subst_first_tac ctxt (List.map (flip_eq_thm ctxt) arg_reg_eq_thms))
-          THEN' Simplifier.asm_simp_tac ctxt (* TODO: narrow simp set *)
-      in
-        instantiate_apply_ih_tac THEN_ALL_NEW SOLVED' solve_ih_prem_tac
-      end
-
-    fun prems_tac {context = ctxt, prems, ...} {s, v, ...} =
-      get_reg_eq_thms ctxt (arg_reg_eq_tac ctxt prems) s v
-      BIND (fn arg_reg_eq_thms =>
-        rewrite_conclusion_arguments_tac ctxt arg_reg_eq_thms
-        THEN' solve_with_ih_tac ctxt prems s arg_reg_eq_thms
-        |> pure)
-      |> flat2
-
-    fun focused_tac ctxt =
-      resolve_tac ctxt [@{thm terminates_with_res_tTailI}]
-      THEN' TU.FOCUS_PREMS' (with_dest_terminates_with_res_IMP_Tailcall_prop o prems_tac) ctxt
-  in
-    TU.FOCUS_PARAMS_CTXT' focused_tac
-  end
-
-fun finish_non_tail_tac ctxt =
-  terminates_with_res_tAssign_tac ctxt
-  THEN' HTIB.STATE_interp_retrieve_key_eq_tac (asm_simp_tac (ctxt addsimps (@{thms Let_def}))) ctxt
-
-
-(* common tail/non-tail finish tactics *)
-
-(* run the HOL function to its return value or to a recursive call *)
-fun run_hol_fun_tac get_HOL_eqs =
-  let fun tac ctxt {v, ...} =
-    case get_HOL_eqs ctxt (head_of v) of
-      NONE => (writeln "Could not find HOL equality for HOL term in conclusion"; (* TODO *) K no_tac)
-    | SOME thms =>
-        HTIU.subst_first_tac ctxt thms
-        (* TODO: the simplification step is fragile if there is any
-          other theorem about the HOL function in the simpset *)
-        (* TODO: target the relevant assumptions only (?) *)
-        THEN' TU.TRY' (Simplifier.asm_simp_tac ctxt)
-  in with_dest_terminates_with_res_IMP_Tailcall_prop o tac end
-
-fun finish_tac get_HOL_eqs =
-  let fun tac ctxt =
-    run_hol_fun_tac get_HOL_eqs ctxt
-    THEN' (finish_tail_tac ctxt ORELSE' finish_non_tail_tac ctxt)
-  in TU.FOCUS_PARAMS_CTXT' tac end
-
-end
-
-structure HA = struct
-open HA
-
-(* chef special *)
-
-fun cook tailcall =
-  let
-    fun tac ctxt =
-      HTIT.preprocess_tac H.get_IMP_def ctxt
-      THEN' (if tailcall then HTIT.setup_induction_tac HA.get_HOL_inducts ctxt else K all_tac)
-      THEN_ALL_NEW (
-        HTIT.start_case_tac H.get_IMP_def ctxt
-        THEN' HTIT.run_tac HTIT.get_func_corrects ctxt
-        THEN_ALL_NEW (
-          HTIT.finish_tac HTIB.get_HOL_eqs ctxt
-          ORELSE' SOLVED' (Simplifier.asm_simp_tac ctxt)
-          ORELSE' K all_tac))
-  in
-    TU.FOCUS_PARAMS_CTXT' tac
-  end
-
-end
-\<close>
-
-HOL_To_IMP_Minus_func_correct mul_acc_nat
-  apply (tactic \<open>HA.cook true @{context} 1\<close>) done
+HOL_To_IMP_Minus_func_correct mul_acc_nat by (cook mode = tailcall)
 
 lemma mul_acc_nat_eq_mul_add[simp]: "mul_acc_nat x y z = x * y + z"
   by (induction x y z arbitrary: z rule: mul_acc_nat.induct)
@@ -503,8 +62,7 @@ compile_nat div_acc_nat.simps basename div_acc
 
 thm div_acc_nat.induct
 
-HOL_To_IMP_Minus_func_correct div_acc_nat
-  apply (tactic \<open>HA.cook true @{context} 1\<close>) done
+HOL_To_IMP_Minus_func_correct div_acc_nat by (cook mode = tailcall)
 
 lemma div_acc_nat_eq_div[simp]: "div_acc_nat x y z = x div y + z"
   by (induction x y z rule: div_acc_nat.induct) (auto simp: div_acc_nat.simps div_if)
@@ -522,16 +80,14 @@ declare_compiled_const "divide"
   argument_registers "div.args.x" "div.args.y"
   compiled "tailcall_to_IMP_Minus div_IMP_tailcall"
 
-HOL_To_IMP_Minus_func_correct div_nat
-  apply (tactic \<open>HA.cook false @{context} 1\<close>) done
+HOL_To_IMP_Minus_func_correct div_nat by cook
 
 definition square_nat :: "nat \<Rightarrow> nat" where
   "square_nat x \<equiv> mul_nat x x"
 
 compile_nat square_nat_def basename square
 
-HOL_To_IMP_Minus_func_correct square_nat
-  apply (tactic \<open>HA.cook false @{context} 1\<close>) done
+HOL_To_IMP_Minus_func_correct square_nat by cook
 
 lemma square_nat_eq_square[simp]: "square_nat x = x\<^sup>2"
   unfolding square_nat_def by (simp add: power2_eq_square)
@@ -552,18 +108,18 @@ declare sqrt_aux_nat.simps[simp del]
 
 compile_nat sqrt_aux_nat.simps basename sqrt_aux
 
-HOL_To_IMP_Minus_func_correct sqrt_aux_nat
-  apply (tactic \<open>HA.cook true @{context} 1\<close>) done
+HOL_To_IMP_Minus_func_correct sqrt_aux_nat by (cook mode = tailcall)
+(* TODO: ignoring duplicate rewrite rule *)
 
 (* Example step-by-step tactic invocation. Do not remove for debugging purposes *)
 HOL_To_IMP_Minus_func_correct sqrt_aux_nat
-  apply (tactic \<open>HTIT.preprocess_tac H.get_IMP_def @{context} 1\<close>)
-  apply (tactic \<open>HTIT.setup_induction_tac HA.get_HOL_inducts @{context} 1\<close>)
-  apply (tactic \<open>HTIT.start_case_tac H.get_IMP_def @{context} 1\<close>)
-  apply (tactic \<open>HTIT.run_tac HTIT.get_func_corrects @{context} 1\<close>)
-  apply (tactic \<open>HTIT.finish_tac HTIB.get_HOL_eqs @{context} 1\<close>)
-  apply (tactic \<open>HTIT.finish_tac HTIB.get_HOL_eqs @{context} 1\<close>)
-  apply (tactic \<open>HTIT.finish_tac HTIB.get_HOL_eqs @{context} 1\<close>)
+  apply (tactic \<open>H.preprocess_tac H.get_IMP_def @{context} 1\<close>)
+  apply (tactic \<open>H.setup_induction_tac HA.get_HOL_inducts @{context} 1\<close>)
+  apply (tactic \<open>H.start_case_tac H.get_IMP_def @{context} 1\<close>)
+  apply (tactic \<open>H.run_tac H.get_func_corrects @{context} 1\<close>)
+  apply (tactic \<open>H.finish_tac HB.get_HOL_eqs @{context} 1\<close>)
+  apply (tactic \<open>H.finish_tac HB.get_HOL_eqs @{context} 1\<close>)
+  apply (tactic \<open>H.finish_tac HB.get_HOL_eqs @{context} 1\<close>)
   oops
 
 lemma square_sqrt_aux_nat_le:
@@ -585,8 +141,7 @@ definition sqrt_nat :: "nat \<Rightarrow> nat" where
 
 compile_nat sqrt_nat_def basename sqrt
 
-HOL_To_IMP_Minus_func_correct sqrt_nat
-  apply (tactic \<open>HA.cook false @{context} 1 \<close>) done
+HOL_To_IMP_Minus_func_correct sqrt_nat by cook
 
 lemma square_sqrt_nat_le: "(sqrt_nat x)\<^sup>2 \<le> x"
   using square_sqrt_aux_nat_le unfolding sqrt_nat_def by (simp add: power2_eq_square)
